Lane Biocini 30 September 2023

The transposition operator, related to inversion

\begin{code}

{-# OPTIONS --without-K --exact-split --safe #-}

module ModularGroup.Transposition where

open import MLTT.Spartan
open import Notation.General

open import ModularGroup.Type
open import ModularGroup.Composition

_áµ€ : ğ“œ â†’ ğ“œ
E áµ€ = E
S áµ€ = S
ğ’” x áµ€ = Î¸ x áµ€ â€¢ S
ğ’“ x áµ€ = Î· x áµ€ â€¢ SRÂ²S
ğ’“Â² x áµ€ = Î· x áµ€ â€¢ SRS

infix 32 _áµ€

is-symmetric : ğ“œ â†’ ğ“¤â‚€ Ì‡
is-symmetric a = a ï¼ a áµ€

ğ“œ-symmetric : ğ“¤â‚€ Ì‡
ğ“œ-symmetric = Î£ a ê‰ ğ“œ , is-symmetric a

transpose-s : (x : ğ“œ) â†’ (s x) áµ€ ï¼ x áµ€ â€¢ S
transpose-s E = refl
transpose-s S = refl
transpose-s (ğ’” x) =
 Î¸ x áµ€           ï¼âŸ¨ compose-right-neutral (Î¸ x áµ€) â»Â¹ âŸ©
 Î¸ x áµ€ â€¢ E       ï¼âŸ¨ compose-associative (Î¸ x áµ€) S S â»Â¹ âŸ©
 (Î¸ x áµ€ â€¢ S) â€¢ S âˆ
transpose-s (Î¸ x) = refl

transpose-r : (x : ğ“œ) â†’ (r x) áµ€ ï¼ x áµ€ â€¢ SRÂ²S
transpose-r (Î· x) = refl
transpose-r (ğ’“ x) = compose-associative (Î· x áµ€) SRÂ²S SRÂ²S â»Â¹
transpose-r (ğ’“Â² x) =
 Î· x áµ€                  ï¼âŸ¨ compose-right-neutral (Î· x áµ€) â»Â¹ âŸ©
 Î· x áµ€ â€¢ E              ï¼âŸ¨ compose-associative (Î· x áµ€) SRS SRÂ²S â»Â¹ âŸ©
 (Î· x áµ€ â€¢ SRS) â€¢ SRÂ²S âˆ

transpose-rÂ² : (x : ğ“œ) â†’ (rÂ² x) áµ€ ï¼ x áµ€ â€¢ s (r S)
transpose-rÂ² (Î· x) = refl
transpose-rÂ² (ğ’“ x) =
 Î· x áµ€                ï¼âŸ¨ compose-right-neutral (Î· x áµ€) â»Â¹ âŸ©
 Î· x áµ€ â€¢ E            ï¼âŸ¨ compose-associative (Î· x áµ€) SRÂ²S SRS â»Â¹ âŸ©
 (Î· x áµ€ â€¢ SRÂ²S) â€¢ SRS âˆ
transpose-rÂ² (ğ’“Â² x) = compose-associative (Î· x áµ€) (sr S) (sr S) â»Â¹

transpose-product : (a b : ğ“œ) â†’ (a â€¢ b) áµ€ ï¼ b áµ€ â€¢ a áµ€
transpose-product E b = compose-right-neutral (b áµ€) â»Â¹
transpose-product S b = transpose-s b
transpose-product (ğ’” x) b =
 s (Î¸ x â€¢ b) áµ€     ï¼âŸ¨ transpose-s (Î¸ x â€¢ b) âŸ©
 (Î¸ x â€¢ b) áµ€ â€¢ S   ï¼âŸ¨ ap (_â€¢ S) (transpose-product (Î¸ x) b) âŸ©
 (b áµ€ â€¢ Î¸ x áµ€) â€¢ S ï¼âŸ¨ compose-associative (b áµ€) (Î¸ x áµ€) S âŸ©
 b áµ€ â€¢ Î¸ x áµ€ â€¢ S   âˆ
transpose-product (ğ’“ x) b =
 r (Î· x â€¢ b) áµ€        ï¼âŸ¨ transpose-r (Î· x â€¢ b) âŸ©
 (Î· x â€¢ b) áµ€ â€¢ SRÂ²S   ï¼âŸ¨ ap (_â€¢ srÂ² S) (transpose-product (Î· x) b ) âŸ©
 (b áµ€ â€¢ Î· x áµ€) â€¢ SRÂ²S ï¼âŸ¨ compose-associative (b áµ€) (Î· x áµ€) SRÂ²S âŸ©
 b áµ€ â€¢ Î· x áµ€ â€¢ SRÂ²S   âˆ
transpose-product (ğ’“Â² x) b = transpose-rÂ² (Î· x â€¢ b)
 âˆ™ (ap (_â€¢ SRS) (transpose-product (Î· x) b)
 âˆ™ compose-associative (b áµ€) (Î· x áµ€) SRS)

transpose-right-s : (x : ğ“œ) â†’ (x â€¢ S) áµ€ ï¼ s (x áµ€)
transpose-right-s x = transpose-product x S

transpose-right-r : (x : ğ“œ) â†’ (x â€¢ R) áµ€ ï¼ srÂ²s (x áµ€ )
transpose-right-r x = transpose-product x R

transpose-right-rÂ² : (x : ğ“œ) â†’ (x â€¢ RÂ²) áµ€ ï¼ srs (x áµ€)
transpose-right-rÂ² x = transpose-product x RÂ²

transpose-involutive : involutive (_áµ€)
transpose-involutive E = refl
transpose-involutive S = refl
transpose-involutive (ğ’” x) =
 (Î¸ x áµ€ â€¢ S) áµ€ ï¼âŸ¨ transpose-product (Î¸ x áµ€) S âŸ©
 s ((Î¸ x áµ€) áµ€) ï¼âŸ¨ ap s (transpose-involutive (Î¸ x)) âŸ©
 ğ’” x           âˆ
transpose-involutive (ğ’“ x) =
 (Î· x áµ€ â€¢ SRÂ²S) áµ€ ï¼âŸ¨ transpose-product (Î· x áµ€) SRÂ²S âŸ©
 r ((Î· x áµ€) áµ€)    ï¼âŸ¨ ap r (transpose-involutive (Î· x)) âŸ©
 ğ’“ x              âˆ
transpose-involutive (ğ’“Â² x) =
 (Î· x áµ€ â€¢ SRS) áµ€   ï¼âŸ¨ transpose-product (Î· x áµ€) SRS âŸ©
 r (r ((Î· x áµ€) áµ€)) ï¼âŸ¨ ap rÂ² (transpose-involutive (Î· x)) âŸ©
 ğ’“Â² x              âˆ

inverse-transpose : (a : ğ“œ) â†’ (a áµ€ -Â¹) ï¼ ((a -Â¹) áµ€)
inverse-transpose E = refl
inverse-transpose S = refl
inverse-transpose (ğ’” x) =
 (Î¸ x áµ€ â€¢ S) -Â¹ ï¼âŸ¨ inverse-product (Î¸ x áµ€) S âŸ©
 s ((Î¸ x áµ€) -Â¹) ï¼âŸ¨ ap s (inverse-transpose (Î¸ x)) âŸ©
 s ((Î¸ x -Â¹) áµ€) ï¼âŸ¨ transpose-product (Î¸ x -Â¹) S â»Â¹ âŸ©
 (Î¸ x -Â¹ â€¢ S) áµ€ âˆ
inverse-transpose (ğ’“ x) =
 (Î· x áµ€ â€¢ SRÂ²S) -Â¹      ï¼âŸ¨ inverse-product (Î· x áµ€) SRÂ²S âŸ©
 s (r (s ((Î· x áµ€) -Â¹))) ï¼âŸ¨ ap srs (inverse-transpose (Î· x)) âŸ©
 s (r (s ((Î· x -Â¹) áµ€))) ï¼âŸ¨ transpose-product (Î· x -Â¹) RÂ² â»Â¹ âŸ©
 (Î· x -Â¹ â€¢ RÂ²) áµ€        âˆ
inverse-transpose (ğ’“Â² x) =
 (Î· x áµ€ â€¢ SRS) -Â¹           ï¼âŸ¨ inverse-product (Î· x áµ€) SRS âŸ©
 s (r (r (s ((Î· x áµ€) -Â¹)))) ï¼âŸ¨ ap srÂ²s (inverse-transpose (Î· x)) âŸ©
 s (r (r (s ((Î· x -Â¹) áµ€)))) ï¼âŸ¨ transpose-product (Î· x -Â¹) R â»Â¹ âŸ©
 (Î· x -Â¹ â€¢ R) áµ€             âˆ

\end{code}
